iris/WpGprCsrw.v
@@ -434,7 +434,7 @@ Section WpCsrwMedeleg.
       (b1 : bool) (npc0 mst0 mstatus0 : mword 64)
       (mc : mword 32) (mcfg : mword 64)
       (pmpcfg0 : type_of_register pmpcfg_n) (pmar0 : list PMA_Region)
-      (mi0 : bool) (elp0 : mword 1) E (Phi : mval -> iProp Σ) :
+      (mi0 : bool) (elp0 : mword 1) E {dq : dfrac} (Phi : mval -> iProp Σ) :
     uint rs1 <> 0 ->
     m !! gpr_of_Z (uint rs1) = Some vrs1 ->
     eq_vec (_get_Misa_S misa0) ('b"1") = true ->
@@ -457,7 +457,7 @@ Section WpCsrwMedeleg.
     (R_bitvector_64 mideleg) ↦ᵣ mdv0 -∗ (R_bitvector_64 mstatus) ↦ᵣ mstatus0 -∗
     elp ↦ᵣ elp0 -∗ mcountinhibit ↦ᵣ mc -∗ minstretcfg ↦ᵣ mcfg -∗
     pmpcfg_n ↦ᵣ pmpcfg0 -∗ pma_regions ↦ᵣ pmar0 -∗ htif_tohost_base ↦ᵣ None -∗
-    ([∗ list] j ∈ seq 0 4, (pa_add (fetch_pa pc) j) ↦ₘ nth_byte w j) -∗
+    ([∗ list] j ∈ seq 0 4, (pa_add (fetch_pa pc) j) ↦ₘ{dq} nth_byte w j) -∗
     ▷ ( PC ↦ᵣ add_vec_int pc 4 -∗ gpr_file m -∗
         medeleg ↦ᵣ legalize_medeleg medeleg0 vrs1 -∗ misa ↦ᵣ misa0 -∗
         nextPC ↦ᵣ add_vec_int pc 4 -∗ (R_bool minstret_increment) ↦ᵣ b1 -∗
@@ -466,7 +466,7 @@ Section WpCsrwMedeleg.
         (R_bitvector_64 mideleg) ↦ᵣ mdv0 -∗ (R_bitvector_64 mstatus) ↦ᵣ mstatus0 -∗
         elp ↦ᵣ elp0 -∗ mcountinhibit ↦ᵣ mc -∗ minstretcfg ↦ᵣ mcfg -∗
         pmpcfg_n ↦ᵣ pmpcfg0 -∗ pma_regions ↦ᵣ pmar0 -∗ htif_tohost_base ↦ᵣ None -∗
-        ([∗ list] j ∈ seq 0 4, (pa_add (fetch_pa pc) j) ↦ₘ nth_byte w j) -∗
+        ([∗ list] j ∈ seq 0 4, (pa_add (fetch_pa pc) j) ↦ₘ{dq} nth_byte w j) -∗
         WP (Loop : expr riscv_lang) @ E {{ Phi }}) -∗
     WP (Loop : expr riscv_lang) @ E {{ Phi }}.
   Proof.
@@ -656,7 +656,7 @@ Section WpCsrwMcounteren.
       (b1 : bool) (npc0 mst0 mstatus0 : mword 64)
       (mc : mword 32) (mcfg : mword 64)
       (pmpcfg0 : type_of_register pmpcfg_n) (pmar0 : list PMA_Region)
-      (mi0 : bool) (elp0 : mword 1) E (Phi : mval -> iProp Σ) :
+      (mi0 : bool) (elp0 : mword 1) E {dq : dfrac} (Phi : mval -> iProp Σ) :
     uint rs1 <> 0 ->
     m !! gpr_of_Z (uint rs1) = Some vrs1 ->
     eq_vec (_get_Misa_S misa0) ('b"1") = true ->
@@ -680,7 +680,7 @@ Section WpCsrwMcounteren.
     (R_bitvector_64 mideleg) ↦ᵣ mdv0 -∗ (R_bitvector_64 mstatus) ↦ᵣ mstatus0 -∗
     elp ↦ᵣ elp0 -∗ mcountinhibit ↦ᵣ mc -∗ minstretcfg ↦ᵣ mcfg -∗
     pmpcfg_n ↦ᵣ pmpcfg0 -∗ pma_regions ↦ᵣ pmar0 -∗ htif_tohost_base ↦ᵣ None -∗
-    ([∗ list] j ∈ seq 0 4, (pa_add (fetch_pa pc) j) ↦ₘ nth_byte w j) -∗
+    ([∗ list] j ∈ seq 0 4, (pa_add (fetch_pa pc) j) ↦ₘ{dq} nth_byte w j) -∗
     ▷ ( PC ↦ᵣ add_vec_int pc 4 -∗ gpr_file m -∗
         mcounteren ↦ᵣ legalize_mcounteren mcounteren0 vrs1 -∗ misa ↦ᵣ misa0 -∗
         nextPC ↦ᵣ add_vec_int pc 4 -∗ (R_bool minstret_increment) ↦ᵣ b1 -∗
@@ -689,7 +689,7 @@ Section WpCsrwMcounteren.
         (R_bitvector_64 mideleg) ↦ᵣ mdv0 -∗ (R_bitvector_64 mstatus) ↦ᵣ mstatus0 -∗
         elp ↦ᵣ elp0 -∗ mcountinhibit ↦ᵣ mc -∗ minstretcfg ↦ᵣ mcfg -∗
         pmpcfg_n ↦ᵣ pmpcfg0 -∗ pma_regions ↦ᵣ pmar0 -∗ htif_tohost_base ↦ᵣ None -∗
-        ([∗ list] j ∈ seq 0 4, (pa_add (fetch_pa pc) j) ↦ₘ nth_byte w j) -∗
+        ([∗ list] j ∈ seq 0 4, (pa_add (fetch_pa pc) j) ↦ₘ{dq} nth_byte w j) -∗
         WP (Loop : expr riscv_lang) @ E {{ Phi }}) -∗
     WP (Loop : expr riscv_lang) @ E {{ Phi }}.
   Proof.
@@ -927,7 +927,7 @@ Section WpCsrwMepc.
       (b1 : bool) (npc0 mst0 mstatus0 : mword 64)
       (mc : mword 32) (mcfg : mword 64)
       (pmpcfg0 : type_of_register pmpcfg_n) (pmar0 : list PMA_Region)
-      (mi0 : bool) (elp0 : mword 1) E (Phi : mval -> iProp Σ) :
+      (mi0 : bool) (elp0 : mword 1) E {dq : dfrac} (Phi : mval -> iProp Σ) :
     uint rs1 <> 0 ->
     m !! gpr_of_Z (uint rs1) = Some vrs1 ->
     eq_vec (_get_Misa_S misa0) ('b"1") = true ->
@@ -950,7 +950,7 @@ Section WpCsrwMepc.
     (R_bitvector_64 mideleg) ↦ᵣ mdv0 -∗ (R_bitvector_64 mstatus) ↦ᵣ mstatus0 -∗
     elp ↦ᵣ elp0 -∗ mcountinhibit ↦ᵣ mc -∗ minstretcfg ↦ᵣ mcfg -∗
     pmpcfg_n ↦ᵣ pmpcfg0 -∗ pma_regions ↦ᵣ pmar0 -∗ htif_tohost_base ↦ᵣ None -∗
-    ([∗ list] j ∈ seq 0 4, (pa_add (fetch_pa pc) j) ↦ₘ nth_byte w j) -∗
+    ([∗ list] j ∈ seq 0 4, (pa_add (fetch_pa pc) j) ↦ₘ{dq} nth_byte w j) -∗
     ▷ ( PC ↦ᵣ add_vec_int pc 4 -∗ gpr_file m -∗
         mepc ↦ᵣ mepc_val vrs1 -∗ misa ↦ᵣ misa0 -∗
         nextPC ↦ᵣ add_vec_int pc 4 -∗ (R_bool minstret_increment) ↦ᵣ b1 -∗
@@ -959,7 +959,7 @@ Section WpCsrwMepc.
         (R_bitvector_64 mideleg) ↦ᵣ mdv0 -∗ (R_bitvector_64 mstatus) ↦ᵣ mstatus0 -∗
         elp ↦ᵣ elp0 -∗ mcountinhibit ↦ᵣ mc -∗ minstretcfg ↦ᵣ mcfg -∗
         pmpcfg_n ↦ᵣ pmpcfg0 -∗ pma_regions ↦ᵣ pmar0 -∗ htif_tohost_base ↦ᵣ None -∗
-        ([∗ list] j ∈ seq 0 4, (pa_add (fetch_pa pc) j) ↦ₘ nth_byte w j) -∗
+        ([∗ list] j ∈ seq 0 4, (pa_add (fetch_pa pc) j) ↦ₘ{dq} nth_byte w j) -∗
         WP (Loop : expr riscv_lang) @ E {{ Phi }}) -∗
     WP (Loop : expr riscv_lang) @ E {{ Phi }}.
   Proof.
@@ -1162,7 +1162,7 @@ Section WpCsrwMscratch.
       (b1 : bool) (npc0 mst0 mstatus0 : mword 64)
       (mc : mword 32) (mcfg : mword 64)
       (pmpcfg0 : type_of_register pmpcfg_n) (pmar0 : list PMA_Region)
-      (mi0 : bool) (elp0 : mword 1) E (Phi : mval -> iProp Σ) :
+      (mi0 : bool) (elp0 : mword 1) E {dq : dfrac} (Phi : mval -> iProp Σ) :
     uint rs1 <> 0 ->
     m !! gpr_of_Z (uint rs1) = Some vrs1 ->
     eq_vec (_get_Misa_S misa0) ('b"1") = true ->
@@ -1185,7 +1185,7 @@ Section WpCsrwMscratch.
     (R_bitvector_64 mideleg) ↦ᵣ mdv0 -∗ (R_bitvector_64 mstatus) ↦ᵣ mstatus0 -∗
     elp ↦ᵣ elp0 -∗ mcountinhibit ↦ᵣ mc -∗ minstretcfg ↦ᵣ mcfg -∗
     pmpcfg_n ↦ᵣ pmpcfg0 -∗ pma_regions ↦ᵣ pmar0 -∗ htif_tohost_base ↦ᵣ None -∗
-    ([∗ list] j ∈ seq 0 4, (pa_add (fetch_pa pc) j) ↦ₘ nth_byte w j) -∗
+    ([∗ list] j ∈ seq 0 4, (pa_add (fetch_pa pc) j) ↦ₘ{dq} nth_byte w j) -∗
     ▷ ( PC ↦ᵣ add_vec_int pc 4 -∗ gpr_file m -∗
         mscratch ↦ᵣ vrs1 -∗ misa ↦ᵣ misa0 -∗
         nextPC ↦ᵣ add_vec_int pc 4 -∗ (R_bool minstret_increment) ↦ᵣ b1 -∗
@@ -1194,7 +1194,7 @@ Section WpCsrwMscratch.
         (R_bitvector_64 mideleg) ↦ᵣ mdv0 -∗ (R_bitvector_64 mstatus) ↦ᵣ mstatus0 -∗
         elp ↦ᵣ elp0 -∗ mcountinhibit ↦ᵣ mc -∗ minstretcfg ↦ᵣ mcfg -∗
         pmpcfg_n ↦ᵣ pmpcfg0 -∗ pma_regions ↦ᵣ pmar0 -∗ htif_tohost_base ↦ᵣ None -∗
-        ([∗ list] j ∈ seq 0 4, (pa_add (fetch_pa pc) j) ↦ₘ nth_byte w j) -∗
+        ([∗ list] j ∈ seq 0 4, (pa_add (fetch_pa pc) j) ↦ₘ{dq} nth_byte w j) -∗
         WP (Loop : expr riscv_lang) @ E {{ Phi }}) -∗
     WP (Loop : expr riscv_lang) @ E {{ Phi }}.
   Proof.
@@ -1508,7 +1508,7 @@ Section WpCsrwMideleg.
       (b1 : bool) (npc0 mst0 mstatus0 : mword 64)
       (mc : mword 32) (mcfg : mword 64)
       (pmpcfg0 : type_of_register pmpcfg_n) (pmar0 : list PMA_Region)
-      (mi0 : bool) (elp0 : mword 1) E (Phi : mval -> iProp Σ) :
+      (mi0 : bool) (elp0 : mword 1) E {dq : dfrac} (Phi : mval -> iProp Σ) :
     uint rs1 <> 0 ->
     m !! gpr_of_Z (uint rs1) = Some vrs1 ->
     eq_vec (_get_Misa_S misa0) ('b"1") = true ->
@@ -1531,7 +1531,7 @@ Section WpCsrwMideleg.
     (R_bitvector_64 mideleg) ↦ᵣ mdv0 -∗ (R_bitvector_64 mstatus) ↦ᵣ mstatus0 -∗
     elp ↦ᵣ elp0 -∗ mcountinhibit ↦ᵣ mc -∗ minstretcfg ↦ᵣ mcfg -∗
     pmpcfg_n ↦ᵣ pmpcfg0 -∗ pma_regions ↦ᵣ pmar0 -∗ htif_tohost_base ↦ᵣ None -∗
-    ([∗ list] j ∈ seq 0 4, (pa_add (fetch_pa pc) j) ↦ₘ nth_byte w j) -∗
+    ([∗ list] j ∈ seq 0 4, (pa_add (fetch_pa pc) j) ↦ₘ{dq} nth_byte w j) -∗
     ▷ ( PC ↦ᵣ add_vec_int pc 4 -∗ gpr_file m -∗ misa ↦ᵣ misa0 -∗
         nextPC ↦ᵣ add_vec_int pc 4 -∗ (R_bool minstret_increment) ↦ᵣ b1 -∗
         minstret ↦ᵣ (if b1 then add_vec_int mst0 1 else mst0) -∗
@@ -1540,7 +1540,7 @@ Section WpCsrwMideleg.
         (R_bitvector_64 mstatus) ↦ᵣ mstatus0 -∗
         elp ↦ᵣ elp0 -∗ mcountinhibit ↦ᵣ mc -∗ minstretcfg ↦ᵣ mcfg -∗
         pmpcfg_n ↦ᵣ pmpcfg0 -∗ pma_regions ↦ᵣ pmar0 -∗ htif_tohost_base ↦ᵣ None -∗
-        ([∗ list] j ∈ seq 0 4, (pa_add (fetch_pa pc) j) ↦ₘ nth_byte w j) -∗
+        ([∗ list] j ∈ seq 0 4, (pa_add (fetch_pa pc) j) ↦ₘ{dq} nth_byte w j) -∗
         WP (Loop : expr riscv_lang) @ E {{ Phi }}) -∗
     WP (Loop : expr riscv_lang) @ E {{ Phi }}.
   Proof.
@@ -1789,7 +1789,7 @@ Section WpCsrwSie.
       (b1 : bool) (npc0 mst0 mstatus0 : mword 64)
       (mc : mword 32) (mcfg : mword 64)
       (pmpcfg0 : type_of_register pmpcfg_n) (pmar0 : list PMA_Region)
-      (mi0 : bool) (elp0 : mword 1) E (Phi : mval -> iProp Σ) :
+      (mi0 : bool) (elp0 : mword 1) E {dq : dfrac} (Phi : mval -> iProp Σ) :
     uint rs1 <> 0 ->
     m !! gpr_of_Z (uint rs1) = Some vrs1 ->
     eq_vec (_get_Misa_S misa0) ('b"1") = true ->
@@ -1812,7 +1812,7 @@ Section WpCsrwSie.
     (R_bitvector_64 mideleg) ↦ᵣ mdv0 -∗ (R_bitvector_64 mstatus) ↦ᵣ mstatus0 -∗
     elp ↦ᵣ elp0 -∗ mcountinhibit ↦ᵣ mc -∗ minstretcfg ↦ᵣ mcfg -∗
     pmpcfg_n ↦ᵣ pmpcfg0 -∗ pma_regions ↦ᵣ pmar0 -∗ htif_tohost_base ↦ᵣ None -∗
-    ([∗ list] j ∈ seq 0 4, (pa_add (fetch_pa pc) j) ↦ₘ nth_byte w j) -∗
+    ([∗ list] j ∈ seq 0 4, (pa_add (fetch_pa pc) j) ↦ₘ{dq} nth_byte w j) -∗
     ▷ ( PC ↦ᵣ add_vec_int pc 4 -∗ gpr_file m -∗
         mie ↦ᵣ sie_new_mie mie0 mdv0 vrs1 -∗ misa ↦ᵣ misa0 -∗
         nextPC ↦ᵣ add_vec_int pc 4 -∗ (R_bool minstret_increment) ↦ᵣ b1 -∗
@@ -1821,7 +1821,7 @@ Section WpCsrwSie.
         (R_bitvector_64 mideleg) ↦ᵣ mdv0 -∗ (R_bitvector_64 mstatus) ↦ᵣ mstatus0 -∗
         elp ↦ᵣ elp0 -∗ mcountinhibit ↦ᵣ mc -∗ minstretcfg ↦ᵣ mcfg -∗
         pmpcfg_n ↦ᵣ pmpcfg0 -∗ pma_regions ↦ᵣ pmar0 -∗ htif_tohost_base ↦ᵣ None -∗
-        ([∗ list] j ∈ seq 0 4, (pa_add (fetch_pa pc) j) ↦ₘ nth_byte w j) -∗
+        ([∗ list] j ∈ seq 0 4, (pa_add (fetch_pa pc) j) ↦ₘ{dq} nth_byte w j) -∗
         WP (Loop : expr riscv_lang) @ E {{ Phi }}) -∗
     WP (Loop : expr riscv_lang) @ E {{ Phi }}.
   Proof.
@@ -2255,7 +2255,7 @@ Section WpCsrwMstatus.
       (b1 : bool) (npc0 mst0 : mword 64)
       (mc : mword 32) (mcfg : mword 64)
       (pmpcfg0 : type_of_register pmpcfg_n) (pmar0 : list PMA_Region)
-      (mi0 : bool) (elp0 : mword 1) E (Phi : mval -> iProp Σ) :
+      (mi0 : bool) (elp0 : mword 1) E {dq : dfrac} (Phi : mval -> iProp Σ) :
     uint rs1 <> 0 ->
     m !! gpr_of_Z (uint rs1) = Some vrs1 ->
     eq_vec (_get_Misa_S misa0) ('b"1") = true ->
@@ -2279,7 +2279,7 @@ Section WpCsrwMstatus.
     (R_bitvector_64 mideleg) ↦ᵣ mdv0 -∗ (R_bitvector_64 mstatus) ↦ᵣ mstatus0 -∗
     elp ↦ᵣ elp0 -∗ mcountinhibit ↦ᵣ mc -∗ minstretcfg ↦ᵣ mcfg -∗
     pmpcfg_n ↦ᵣ pmpcfg0 -∗ pma_regions ↦ᵣ pmar0 -∗ htif_tohost_base ↦ᵣ None -∗
-    ([∗ list] j ∈ seq 0 4, (pa_add (fetch_pa pc) j) ↦ₘ nth_byte w j) -∗
+    ([∗ list] j ∈ seq 0 4, (pa_add (fetch_pa pc) j) ↦ₘ{dq} nth_byte w j) -∗
     ▷ ( PC ↦ᵣ add_vec_int pc 4 -∗ gpr_file m -∗ misa ↦ᵣ misa0 -∗
         nextPC ↦ᵣ add_vec_int pc 4 -∗ (R_bool minstret_increment) ↦ᵣ b1 -∗
         minstret ↦ᵣ (if b1 then add_vec_int mst0 1 else mst0) -∗
@@ -2288,7 +2288,7 @@ Section WpCsrwMstatus.
         (R_bitvector_64 mstatus) ↦ᵣ mstatus_legalized mstatus0 vrs1 -∗
         elp ↦ᵣ elp0 -∗ mcountinhibit ↦ᵣ mc -∗ minstretcfg ↦ᵣ mcfg -∗
         pmpcfg_n ↦ᵣ pmpcfg0 -∗ pma_regions ↦ᵣ pmar0 -∗ htif_tohost_base ↦ᵣ None -∗
-        ([∗ list] j ∈ seq 0 4, (pa_add (fetch_pa pc) j) ↦ₘ nth_byte w j) -∗
+        ([∗ list] j ∈ seq 0 4, (pa_add (fetch_pa pc) j) ↦ₘ{dq} nth_byte w j) -∗
         WP (Loop : expr riscv_lang) @ E {{ Phi }}) -∗
     WP (Loop : expr riscv_lang) @ E {{ Phi }}.
   Proof.
@@ -2680,7 +2680,7 @@ Section WpCsrwSatp.
       (b1 : bool) (npc0 mst0 : mword 64)
       (mc : mword 32) (mcfg : mword 64)
       (pmpcfg0 : type_of_register pmpcfg_n) (pmar0 : list PMA_Region)
-      (mi0 : bool) (elp0 : mword 1) E (Phi : mval -> iProp Σ) :
+      (mi0 : bool) (elp0 : mword 1) E {dq : dfrac} (Phi : mval -> iProp Σ) :
     uint rs1 <> 0 ->
     m !! gpr_of_Z (uint rs1) = Some vrs1 ->
     eq_vec (_get_Misa_S misa0) ('b"1") = true ->
@@ -2704,7 +2704,7 @@ Section WpCsrwSatp.
     (R_bitvector_64 mideleg) ↦ᵣ mdv0 -∗ (R_bitvector_64 mstatus) ↦ᵣ mstatus0 -∗
     elp ↦ᵣ elp0 -∗ mcountinhibit ↦ᵣ mc -∗ minstretcfg ↦ᵣ mcfg -∗
     pmpcfg_n ↦ᵣ pmpcfg0 -∗ pma_regions ↦ᵣ pmar0 -∗ htif_tohost_base ↦ᵣ None -∗
-    ([∗ list] j ∈ seq 0 4, (pa_add (fetch_pa pc) j) ↦ₘ nth_byte w j) -∗
+    ([∗ list] j ∈ seq 0 4, (pa_add (fetch_pa pc) j) ↦ₘ{dq} nth_byte w j) -∗
     ▷ ( PC ↦ᵣ add_vec_int pc 4 -∗ gpr_file m -∗
         satp ↦ᵣ satp_legalized satp0 vrs1 -∗ misa ↦ᵣ misa0 -∗
         nextPC ↦ᵣ add_vec_int pc 4 -∗ (R_bool minstret_increment) ↦ᵣ b1 -∗
@@ -2713,7 +2713,7 @@ Section WpCsrwSatp.
         (R_bitvector_64 mideleg) ↦ᵣ mdv0 -∗ (R_bitvector_64 mstatus) ↦ᵣ mstatus0 -∗
         elp ↦ᵣ elp0 -∗ mcountinhibit ↦ᵣ mc -∗ minstretcfg ↦ᵣ mcfg -∗
         pmpcfg_n ↦ᵣ pmpcfg0 -∗ pma_regions ↦ᵣ pmar0 -∗ htif_tohost_base ↦ᵣ None -∗
-        ([∗ list] j ∈ seq 0 4, (pa_add (fetch_pa pc) j) ↦ₘ nth_byte w j) -∗
+        ([∗ list] j ∈ seq 0 4, (pa_add (fetch_pa pc) j) ↦ₘ{dq} nth_byte w j) -∗
         WP (Loop : expr riscv_lang) @ E {{ Phi }}) -∗
     WP (Loop : expr riscv_lang) @ E {{ Phi }}.
   Proof.
@@ -3027,7 +3027,7 @@ Section WpCsrwPmpaddr0.
       (mc : mword 32) (mcfg : mword 64)
       (pmpcfg0 : type_of_register pmpcfg_n) (pmpaddr00 : type_of_register pmpaddr_n)
       (pmar0 : list PMA_Region)
-      (mi0 : bool) (elp0 : mword 1) E (Phi : mval -> iProp Σ) :
+      (mi0 : bool) (elp0 : mword 1) E {dq : dfrac} (Phi : mval -> iProp Σ) :
     uint rs1 <> 0 ->
     m !! gpr_of_Z (uint rs1) = Some vrs1 ->
     eq_vec (_get_Misa_S misa0) ('b"1") = true ->
@@ -3050,7 +3050,7 @@ Section WpCsrwPmpaddr0.
     (R_bitvector_64 mideleg) ↦ᵣ mdv0 -∗ (R_bitvector_64 mstatus) ↦ᵣ mstatus0 -∗
     elp ↦ᵣ elp0 -∗ mcountinhibit ↦ᵣ mc -∗ minstretcfg ↦ᵣ mcfg -∗
     pmpcfg_n ↦ᵣ pmpcfg0 -∗ pma_regions ↦ᵣ pmar0 -∗ htif_tohost_base ↦ᵣ None -∗
-    ([∗ list] j ∈ seq 0 4, (pa_add (fetch_pa pc) j) ↦ₘ nth_byte w j) -∗
+    ([∗ list] j ∈ seq 0 4, (pa_add (fetch_pa pc) j) ↦ₘ{dq} nth_byte w j) -∗
     ▷ ( PC ↦ᵣ add_vec_int pc 4 -∗ gpr_file m -∗
         pmpaddr_n ↦ᵣ pmp0_newaddr pmpcfg0 pmpaddr00 vrs1 -∗ misa ↦ᵣ misa0 -∗
         nextPC ↦ᵣ add_vec_int pc 4 -∗ (R_bool minstret_increment) ↦ᵣ b1 -∗
@@ -3059,7 +3059,7 @@ Section WpCsrwPmpaddr0.
         (R_bitvector_64 mideleg) ↦ᵣ mdv0 -∗ (R_bitvector_64 mstatus) ↦ᵣ mstatus0 -∗
         elp ↦ᵣ elp0 -∗ mcountinhibit ↦ᵣ mc -∗ minstretcfg ↦ᵣ mcfg -∗
         pmpcfg_n ↦ᵣ pmpcfg0 -∗ pma_regions ↦ᵣ pmar0 -∗ htif_tohost_base ↦ᵣ None -∗
-        ([∗ list] j ∈ seq 0 4, (pa_add (fetch_pa pc) j) ↦ₘ nth_byte w j) -∗
+        ([∗ list] j ∈ seq 0 4, (pa_add (fetch_pa pc) j) ↦ₘ{dq} nth_byte w j) -∗
         WP (Loop : expr riscv_lang) @ E {{ Phi }}) -∗
     WP (Loop : expr riscv_lang) @ E {{ Phi }}.
   Proof.
@@ -3430,7 +3430,7 @@ Section WpCsrwPmpcfg0.
       (b1 : bool) (npc0 mst0 mstatus0 : mword 64)
       (mc : mword 32) (mcfg : mword 64)
       (pmpcfg0 : type_of_register pmpcfg_n) (pmar0 : list PMA_Region)
-      (mi0 : bool) (elp0 : mword 1) E (Phi : mval -> iProp Σ) :
+      (mi0 : bool) (elp0 : mword 1) E {dq : dfrac} (Phi : mval -> iProp Σ) :
     uint rs1 <> 0 ->
     m !! gpr_of_Z (uint rs1) = Some vrs1 ->
     eq_vec (_get_Misa_S misa0) ('b"1") = true ->
@@ -3453,7 +3453,7 @@ Section WpCsrwPmpcfg0.
     (R_bitvector_64 mideleg) ↦ᵣ mdv0 -∗ (R_bitvector_64 mstatus) ↦ᵣ mstatus0 -∗
     elp ↦ᵣ elp0 -∗ mcountinhibit ↦ᵣ mc -∗ minstretcfg ↦ᵣ mcfg -∗
     pmpcfg_n ↦ᵣ pmpcfg0 -∗ pma_regions ↦ᵣ pmar0 -∗ htif_tohost_base ↦ᵣ None -∗
-    ([∗ list] j ∈ seq 0 4, (pa_add (fetch_pa pc) j) ↦ₘ nth_byte w j) -∗
+    ([∗ list] j ∈ seq 0 4, (pa_add (fetch_pa pc) j) ↦ₘ{dq} nth_byte w j) -∗
     ▷ ( PC ↦ᵣ add_vec_int pc 4 -∗ gpr_file m -∗ misa ↦ᵣ misa0 -∗
         nextPC ↦ᵣ add_vec_int pc 4 -∗ (R_bool minstret_increment) ↦ᵣ b1 -∗
         minstret ↦ᵣ (if b1 then add_vec_int mst0 1 else mst0) -∗
@@ -3461,7 +3461,7 @@ Section WpCsrwPmpcfg0.
         (R_bitvector_64 mideleg) ↦ᵣ mdv0 -∗ (R_bitvector_64 mstatus) ↦ᵣ mstatus0 -∗
         elp ↦ᵣ elp0 -∗ mcountinhibit ↦ᵣ mc -∗ minstretcfg ↦ᵣ mcfg -∗
         pmpcfg_n ↦ᵣ pmpcfg0_finalvec vrs1 pmpcfg0 -∗ pma_regions ↦ᵣ pmar0 -∗ htif_tohost_base ↦ᵣ None -∗
-        ([∗ list] j ∈ seq 0 4, (pa_add (fetch_pa pc) j) ↦ₘ nth_byte w j) -∗
+        ([∗ list] j ∈ seq 0 4, (pa_add (fetch_pa pc) j) ↦ₘ{dq} nth_byte w j) -∗
         WP (Loop : expr riscv_lang) @ E {{ Phi }}) -∗
     WP (Loop : expr riscv_lang) @ E {{ Phi }}.
   Proof.
@@ -3533,7 +3533,7 @@ Section WpCsrw2.
       (b1 : bool) (npc0 mst0 : mword 64)
       (mc : mword 32) (mcfg : mword 64)
       (pmpcfg0 : type_of_register pmpcfg_n) (pmar0 : list PMA_Region)
-      (mi0 : bool) (elp0 : mword 1) E (Phi : mval -> iProp Σ) :
+      (mi0 : bool) (elp0 : mword 1) E {dq : dfrac} (Phi : mval -> iProp Σ) :
     uint rs1 <> 0 ->
     m !! gpr_of_Z (uint rs1) = Some vrs1 ->
     eq_vec (_get_Misa_S misa0) ('b"1") = true ->
@@ -3566,7 +3566,7 @@ Section WpCsrw2.
     (R_bitvector_64 mideleg) ↦ᵣ mdv0 -∗ (R_bitvector_64 mstatus) ↦ᵣ mstatus0 -∗
     elp ↦ᵣ elp0 -∗ mcountinhibit ↦ᵣ mc -∗ minstretcfg ↦ᵣ mcfg -∗
     pmpcfg_n ↦ᵣ pmpcfg0 -∗ pma_regions ↦ᵣ pmar0 -∗ htif_tohost_base ↦ᵣ None -∗
-    ([∗ list] j ∈ seq 0 4, (pa_add (fetch_pa pc) j) ↦ₘ nth_byte w j) -∗
+    ([∗ list] j ∈ seq 0 4, (pa_add (fetch_pa pc) j) ↦ₘ{dq} nth_byte w j) -∗
     ▷ ( PC ↦ᵣ add_vec_int pc 4 -∗ gpr_file m -∗
         satp ↦ᵣ satp_legalized satp0 vrs1 -∗ misa ↦ᵣ misa0 -∗
         nextPC ↦ᵣ add_vec_int pc 4 -∗ (R_bool minstret_increment) ↦ᵣ b1 -∗
@@ -3575,7 +3575,7 @@ Section WpCsrw2.
         (R_bitvector_64 mideleg) ↦ᵣ mdv0 -∗ (R_bitvector_64 mstatus) ↦ᵣ mstatus0 -∗
         elp ↦ᵣ elp0 -∗ mcountinhibit ↦ᵣ mc -∗ minstretcfg ↦ᵣ mcfg -∗
         pmpcfg_n ↦ᵣ pmpcfg0 -∗ pma_regions ↦ᵣ pmar0 -∗ htif_tohost_base ↦ᵣ None -∗
-        ([∗ list] j ∈ seq 0 4, (pa_add (fetch_pa pc) j) ↦ₘ nth_byte w j) -∗
+        ([∗ list] j ∈ seq 0 4, (pa_add (fetch_pa pc) j) ↦ₘ{dq} nth_byte w j) -∗
         WP (Loop : expr riscv_lang) @ E {{ Phi }}) -∗
     WP (Loop : expr riscv_lang) @ E {{ Phi }}.
   Proof.
@@ -3646,7 +3646,7 @@ Section WpCsrw2More.
       (b1 : bool) (npc0 mst0 mstatus0 : mword 64)
       (mc : mword 32) (mcfg : mword 64)
       (pmpcfg0 : type_of_register pmpcfg_n) (pmar0 : list PMA_Region)
-      (mi0 : bool) (elp0 : mword 1) E (Phi : mval -> iProp Σ) :
+      (mi0 : bool) (elp0 : mword 1) E {dq : dfrac} (Phi : mval -> iProp Σ) :
     uint rs1 <> 0 ->
     m !! gpr_of_Z (uint rs1) = Some vrs1 ->
     eq_vec (_get_Misa_S misa0) ('b"1") = true ->
@@ -3678,7 +3678,7 @@ Section WpCsrw2More.
     (R_bitvector_64 mideleg) ↦ᵣ mdv0 -∗ (R_bitvector_64 mstatus) ↦ᵣ mstatus0 -∗
     elp ↦ᵣ elp0 -∗ mcountinhibit ↦ᵣ mc -∗ minstretcfg ↦ᵣ mcfg -∗
     pmpcfg_n ↦ᵣ pmpcfg0 -∗ pma_regions ↦ᵣ pmar0 -∗ htif_tohost_base ↦ᵣ None -∗
-    ([∗ list] j ∈ seq 0 4, (pa_add (fetch_pa pc) j) ↦ₘ nth_byte w j) -∗
+    ([∗ list] j ∈ seq 0 4, (pa_add (fetch_pa pc) j) ↦ₘ{dq} nth_byte w j) -∗
     ▷ ( PC ↦ᵣ add_vec_int pc 4 -∗ gpr_file m -∗
         medeleg ↦ᵣ legalize_medeleg medeleg0 vrs1 -∗ misa ↦ᵣ misa0 -∗
         nextPC ↦ᵣ add_vec_int pc 4 -∗ (R_bool minstret_increment) ↦ᵣ b1 -∗
@@ -3687,7 +3687,7 @@ Section WpCsrw2More.
         (R_bitvector_64 mideleg) ↦ᵣ mdv0 -∗ (R_bitvector_64 mstatus) ↦ᵣ mstatus0 -∗
         elp ↦ᵣ elp0 -∗ mcountinhibit ↦ᵣ mc -∗ minstretcfg ↦ᵣ mcfg -∗
         pmpcfg_n ↦ᵣ pmpcfg0 -∗ pma_regions ↦ᵣ pmar0 -∗ htif_tohost_base ↦ᵣ None -∗
-        ([∗ list] j ∈ seq 0 4, (pa_add (fetch_pa pc) j) ↦ₘ nth_byte w j) -∗
+        ([∗ list] j ∈ seq 0 4, (pa_add (fetch_pa pc) j) ↦ₘ{dq} nth_byte w j) -∗
         WP (Loop : expr riscv_lang) @ E {{ Phi }}) -∗
     WP (Loop : expr riscv_lang) @ E {{ Phi }}.
   Proof.
@@ -3753,7 +3753,7 @@ Section WpCsrw2More.
       (b1 : bool) (npc0 mst0 mstatus0 : mword 64)
       (mc : mword 32) (mcfg : mword 64)
       (pmpcfg0 : type_of_register pmpcfg_n) (pmar0 : list PMA_Region)
-      (mi0 : bool) (elp0 : mword 1) E (Phi : mval -> iProp Σ) :
+      (mi0 : bool) (elp0 : mword 1) E {dq : dfrac} (Phi : mval -> iProp Σ) :
     uint rs1 <> 0 ->
     m !! gpr_of_Z (uint rs1) = Some vrs1 ->
     eq_vec (_get_Misa_S misa0) ('b"1") = true ->
@@ -3785,7 +3785,7 @@ Section WpCsrw2More.
     (R_bitvector_64 mideleg) ↦ᵣ mdv0 -∗ (R_bitvector_64 mstatus) ↦ᵣ mstatus0 -∗
     elp ↦ᵣ elp0 -∗ mcountinhibit ↦ᵣ mc -∗ minstretcfg ↦ᵣ mcfg -∗
     pmpcfg_n ↦ᵣ pmpcfg0 -∗ pma_regions ↦ᵣ pmar0 -∗ htif_tohost_base ↦ᵣ None -∗
-    ([∗ list] j ∈ seq 0 4, (pa_add (fetch_pa pc) j) ↦ₘ nth_byte w j) -∗
+    ([∗ list] j ∈ seq 0 4, (pa_add (fetch_pa pc) j) ↦ₘ{dq} nth_byte w j) -∗
     ▷ ( PC ↦ᵣ add_vec_int pc 4 -∗ gpr_file m -∗ misa ↦ᵣ misa0 -∗
         nextPC ↦ᵣ add_vec_int pc 4 -∗ (R_bool minstret_increment) ↦ᵣ b1 -∗
         minstret ↦ᵣ (if b1 then add_vec_int mst0 1 else mst0) -∗
@@ -3794,7 +3794,7 @@ Section WpCsrw2More.
         (R_bitvector_64 mstatus) ↦ᵣ mstatus0 -∗
         elp ↦ᵣ elp0 -∗ mcountinhibit ↦ᵣ mc -∗ minstretcfg ↦ᵣ mcfg -∗
         pmpcfg_n ↦ᵣ pmpcfg0 -∗ pma_regions ↦ᵣ pmar0 -∗ htif_tohost_base ↦ᵣ None -∗
-        ([∗ list] j ∈ seq 0 4, (pa_add (fetch_pa pc) j) ↦ₘ nth_byte w j) -∗
+        ([∗ list] j ∈ seq 0 4, (pa_add (fetch_pa pc) j) ↦ₘ{dq} nth_byte w j) -∗
         WP (Loop : expr riscv_lang) @ E {{ Phi }}) -∗
     WP (Loop : expr riscv_lang) @ E {{ Phi }}.
   Proof.
@@ -3859,7 +3859,7 @@ Section WpCsrw2More.
       (b1 : bool) (npc0 mst0 mstatus0 : mword 64)
       (mc : mword 32) (mcfg : mword 64)
       (pmpcfg0 : type_of_register pmpcfg_n) (pmar0 : list PMA_Region)
-      (mi0 : bool) (elp0 : mword 1) E (Phi : mval -> iProp Σ) :
+      (mi0 : bool) (elp0 : mword 1) E {dq : dfrac} (Phi : mval -> iProp Σ) :
     uint rs1 <> 0 ->
     m !! gpr_of_Z (uint rs1) = Some vrs1 ->
     eq_vec (_get_Misa_S misa0) ('b"1") = true ->
@@ -3891,7 +3891,7 @@ Section WpCsrw2More.
     (R_bitvector_64 mideleg) ↦ᵣ mdv0 -∗ (R_bitvector_64 mstatus) ↦ᵣ mstatus0 -∗
     elp ↦ᵣ elp0 -∗ mcountinhibit ↦ᵣ mc -∗ minstretcfg ↦ᵣ mcfg -∗
     pmpcfg_n ↦ᵣ pmpcfg0 -∗ pma_regions ↦ᵣ pmar0 -∗ htif_tohost_base ↦ᵣ None -∗
-    ([∗ list] j ∈ seq 0 4, (pa_add (fetch_pa pc) j) ↦ₘ nth_byte w j) -∗
+    ([∗ list] j ∈ seq 0 4, (pa_add (fetch_pa pc) j) ↦ₘ{dq} nth_byte w j) -∗
     ▷ ( PC ↦ᵣ add_vec_int pc 4 -∗ gpr_file m -∗
         mie ↦ᵣ sie_new_mie mie0 mdv0 vrs1 -∗ misa ↦ᵣ misa0 -∗
         nextPC ↦ᵣ add_vec_int pc 4 -∗ (R_bool minstret_increment) ↦ᵣ b1 -∗
@@ -3900,7 +3900,7 @@ Section WpCsrw2More.
         (R_bitvector_64 mideleg) ↦ᵣ mdv0 -∗ (R_bitvector_64 mstatus) ↦ᵣ mstatus0 -∗
         elp ↦ᵣ elp0 -∗ mcountinhibit ↦ᵣ mc -∗ minstretcfg ↦ᵣ mcfg -∗
         pmpcfg_n ↦ᵣ pmpcfg0 -∗ pma_regions ↦ᵣ pmar0 -∗ htif_tohost_base ↦ᵣ None -∗
-        ([∗ list] j ∈ seq 0 4, (pa_add (fetch_pa pc) j) ↦ₘ nth_byte w j) -∗
+        ([∗ list] j ∈ seq 0 4, (pa_add (fetch_pa pc) j) ↦ₘ{dq} nth_byte w j) -∗
         WP (Loop : expr riscv_lang) @ E {{ Phi }}) -∗
     WP (Loop : expr riscv_lang) @ E {{ Phi }}.
   Proof.
@@ -3974,7 +3974,7 @@ Section WpCsrw2Pmp.
       (mc : mword 32) (mcfg : mword 64)
       (pmpcfg0 : type_of_register pmpcfg_n) (pmpaddr00 : type_of_register pmpaddr_n)
       (pmar0 : list PMA_Region)
-      (mi0 : bool) (elp0 : mword 1) E (Phi : mval -> iProp Σ) :
+      (mi0 : bool) (elp0 : mword 1) E {dq : dfrac} (Phi : mval -> iProp Σ) :
     uint rs1 <> 0 ->
     m !! gpr_of_Z (uint rs1) = Some vrs1 ->
     eq_vec (_get_Misa_S misa0) ('b"1") = true ->
@@ -4006,7 +4006,7 @@ Section WpCsrw2Pmp.
     (R_bitvector_64 mideleg) ↦ᵣ mdv0 -∗ (R_bitvector_64 mstatus) ↦ᵣ mstatus0 -∗
     elp ↦ᵣ elp0 -∗ mcountinhibit ↦ᵣ mc -∗ minstretcfg ↦ᵣ mcfg -∗
     pmpcfg_n ↦ᵣ pmpcfg0 -∗ pma_regions ↦ᵣ pmar0 -∗ htif_tohost_base ↦ᵣ None -∗
-    ([∗ list] j ∈ seq 0 4, (pa_add (fetch_pa pc) j) ↦ₘ nth_byte w j) -∗
+    ([∗ list] j ∈ seq 0 4, (pa_add (fetch_pa pc) j) ↦ₘ{dq} nth_byte w j) -∗
     ▷ ( PC ↦ᵣ add_vec_int pc 4 -∗ gpr_file m -∗
         pmpaddr_n ↦ᵣ pmp0_newaddr pmpcfg0 pmpaddr00 vrs1 -∗ misa ↦ᵣ misa0 -∗
         nextPC ↦ᵣ add_vec_int pc 4 -∗ (R_bool minstret_increment) ↦ᵣ b1 -∗
@@ -4015,7 +4015,7 @@ Section WpCsrw2Pmp.
         (R_bitvector_64 mideleg) ↦ᵣ mdv0 -∗ (R_bitvector_64 mstatus) ↦ᵣ mstatus0 -∗
         elp ↦ᵣ elp0 -∗ mcountinhibit ↦ᵣ mc -∗ minstretcfg ↦ᵣ mcfg -∗
         pmpcfg_n ↦ᵣ pmpcfg0 -∗ pma_regions ↦ᵣ pmar0 -∗ htif_tohost_base ↦ᵣ None -∗
-        ([∗ list] j ∈ seq 0 4, (pa_add (fetch_pa pc) j) ↦ₘ nth_byte w j) -∗
+        ([∗ list] j ∈ seq 0 4, (pa_add (fetch_pa pc) j) ↦ₘ{dq} nth_byte w j) -∗
         WP (Loop : expr riscv_lang) @ E {{ Phi }}) -∗
     WP (Loop : expr riscv_lang) @ E {{ Phi }}.
   Proof.
@@ -4508,7 +4508,7 @@ Section WpCsrwMenvcfg.
       (b1 : bool) (npc0 mst0 : mword 64)
       (mc : mword 32) (mcfg : mword 64)
       (pmpcfg0 : type_of_register pmpcfg_n) (pmar0 : list PMA_Region)
-      (mi0 : bool) (elp0 : mword 1) E (Phi : mval -> iProp Σ) :
+      (mi0 : bool) (elp0 : mword 1) E {dq : dfrac} (Phi : mval -> iProp Σ) :
     uint rs1 <> 0 ->
     m !! gpr_of_Z (uint rs1) = Some vrs1 ->
     eq_vec (_get_Misa_S misa0) ('b"1") = true ->
@@ -4532,7 +4532,7 @@ Section WpCsrwMenvcfg.
     (R_bitvector_64 mideleg) ↦ᵣ mdv0 -∗ (R_bitvector_64 mstatus) ↦ᵣ mstatus0 -∗
     elp ↦ᵣ elp0 -∗ mcountinhibit ↦ᵣ mc -∗ minstretcfg ↦ᵣ mcfg -∗
     pmpcfg_n ↦ᵣ pmpcfg0 -∗ pma_regions ↦ᵣ pmar0 -∗ htif_tohost_base ↦ᵣ None -∗
-    ([∗ list] j ∈ seq 0 4, (pa_add (fetch_pa pc) j) ↦ₘ nth_byte w j) -∗
+    ([∗ list] j ∈ seq 0 4, (pa_add (fetch_pa pc) j) ↦ₘ{dq} nth_byte w j) -∗
     ▷ ( PC ↦ᵣ add_vec_int pc 4 -∗ gpr_file m -∗
         menvcfg ↦ᵣ menvcfg_legalized menvcfg0 vrs1 -∗ misa ↦ᵣ misa0 -∗
         nextPC ↦ᵣ add_vec_int pc 4 -∗ (R_bool minstret_increment) ↦ᵣ b1 -∗
@@ -4541,7 +4541,7 @@ Section WpCsrwMenvcfg.
         (R_bitvector_64 mideleg) ↦ᵣ mdv0 -∗ (R_bitvector_64 mstatus) ↦ᵣ mstatus0 -∗
         elp ↦ᵣ elp0 -∗ mcountinhibit ↦ᵣ mc -∗ minstretcfg ↦ᵣ mcfg -∗
         pmpcfg_n ↦ᵣ pmpcfg0 -∗ pma_regions ↦ᵣ pmar0 -∗ htif_tohost_base ↦ᵣ None -∗
-        ([∗ list] j ∈ seq 0 4, (pa_add (fetch_pa pc) j) ↦ₘ nth_byte w j) -∗
+        ([∗ list] j ∈ seq 0 4, (pa_add (fetch_pa pc) j) ↦ₘ{dq} nth_byte w j) -∗
         WP (Loop : expr riscv_lang) @ E {{ Phi }}) -∗
     WP (Loop : expr riscv_lang) @ E {{ Phi }}.
   Proof.
@@ -4814,7 +4814,7 @@ Section WpCsrwStimecmp.
       (b1 : bool) (npc0 mst0 : mword 64)
       (mc : mword 32) (mcfg : mword 64)
       (pmpcfg0 : type_of_register pmpcfg_n) (pmar0 : list PMA_Region)
-      (mi0 : bool) (elp0 : mword 1) E (Phi : mval -> iProp Σ) :
+      (mi0 : bool) (elp0 : mword 1) E {dq : dfrac} (Phi : mval -> iProp Σ) :
     uint rs1 <> 0 ->
     m !! gpr_of_Z (uint rs1) = Some vrs1 ->
     eq_vec (_get_Misa_S misa0) ('b"1") = true ->
@@ -4837,7 +4837,7 @@ Section WpCsrwStimecmp.
     (R_bitvector_64 mideleg) ↦ᵣ mdv0 -∗ (R_bitvector_64 mstatus) ↦ᵣ mstatus0 -∗
     elp ↦ᵣ elp0 -∗ mcountinhibit ↦ᵣ mc -∗ minstretcfg ↦ᵣ mcfg -∗
     pmpcfg_n ↦ᵣ pmpcfg0 -∗ pma_regions ↦ᵣ pmar0 -∗ htif_tohost_base ↦ᵣ None -∗
-    ([∗ list] j ∈ seq 0 4, (pa_add (fetch_pa pc) j) ↦ₘ nth_byte w j) -∗
+    ([∗ list] j ∈ seq 0 4, (pa_add (fetch_pa pc) j) ↦ₘ{dq} nth_byte w j) -∗
     ▷ ( PC ↦ᵣ add_vec_int pc 4 -∗ gpr_file m -∗
         stimecmp ↦ᵣ stimecmp_legalized stimecmp0 vrs1 -∗ misa ↦ᵣ misa0 -∗
         nextPC ↦ᵣ add_vec_int pc 4 -∗ (R_bool minstret_increment) ↦ᵣ b1 -∗
@@ -4846,7 +4846,7 @@ Section WpCsrwStimecmp.
         (R_bitvector_64 mideleg) ↦ᵣ mdv0 -∗ (R_bitvector_64 mstatus) ↦ᵣ mstatus0 -∗
         elp ↦ᵣ elp0 -∗ mcountinhibit ↦ᵣ mc -∗ minstretcfg ↦ᵣ mcfg -∗
         pmpcfg_n ↦ᵣ pmpcfg0 -∗ pma_regions ↦ᵣ pmar0 -∗ htif_tohost_base ↦ᵣ None -∗
-        ([∗ list] j ∈ seq 0 4, (pa_add (fetch_pa pc) j) ↦ₘ nth_byte w j) -∗
+        ([∗ list] j ∈ seq 0 4, (pa_add (fetch_pa pc) j) ↦ₘ{dq} nth_byte w j) -∗
         WP (Loop : expr riscv_lang) @ E {{ Phi }}) -∗
     WP (Loop : expr riscv_lang) @ E {{ Phi }}.
   Proof.
@@ -4920,7 +4920,7 @@ Section WpCsrw2Probe.
       (b1 : bool) (npc0 mst0 : mword 64)
       (mc : mword 32) (mcfg : mword 64)
       (pmpcfg0 : type_of_register pmpcfg_n) (pmar0 : list PMA_Region)
-      (mi0 : bool) (elp0 : mword 1) E (Phi : mval -> iProp Σ) :
+      (mi0 : bool) (elp0 : mword 1) E {dq : dfrac} (Phi : mval -> iProp Σ) :
     uint rs1 <> 0 ->
     m !! gpr_of_Z (uint rs1) = Some vrs1 ->
     eq_vec (_get_Misa_S misa0) ('b"1") = true ->
@@ -4953,7 +4953,7 @@ Section WpCsrw2Probe.
     (R_bitvector_64 mideleg) ↦ᵣ mdv0 -∗ (R_bitvector_64 mstatus) ↦ᵣ mstatus0 -∗
     elp ↦ᵣ elp0 -∗ mcountinhibit ↦ᵣ mc -∗ minstretcfg ↦ᵣ mcfg -∗
     pmpcfg_n ↦ᵣ pmpcfg0 -∗ pma_regions ↦ᵣ pmar0 -∗ htif_tohost_base ↦ᵣ None -∗
-    ([∗ list] j ∈ seq 0 4, (pa_add (fetch_pa pc) j) ↦ₘ nth_byte w j) -∗
+    ([∗ list] j ∈ seq 0 4, (pa_add (fetch_pa pc) j) ↦ₘ{dq} nth_byte w j) -∗
     ▷ ( PC ↦ᵣ add_vec_int pc 4 -∗ gpr_file m -∗
         menvcfg ↦ᵣ menvcfg_legalized menvcfg0 vrs1 -∗ misa ↦ᵣ misa0 -∗
         nextPC ↦ᵣ add_vec_int pc 4 -∗ (R_bool minstret_increment) ↦ᵣ b1 -∗
@@ -4962,7 +4962,7 @@ Section WpCsrw2Probe.
         (R_bitvector_64 mideleg) ↦ᵣ mdv0 -∗ (R_bitvector_64 mstatus) ↦ᵣ mstatus0 -∗
         elp ↦ᵣ elp0 -∗ mcountinhibit ↦ᵣ mc -∗ minstretcfg ↦ᵣ mcfg -∗
         pmpcfg_n ↦ᵣ pmpcfg0 -∗ pma_regions ↦ᵣ pmar0 -∗ htif_tohost_base ↦ᵣ None -∗
-        ([∗ list] j ∈ seq 0 4, (pa_add (fetch_pa pc) j) ↦ₘ nth_byte w j) -∗
+        ([∗ list] j ∈ seq 0 4, (pa_add (fetch_pa pc) j) ↦ₘ{dq} nth_byte w j) -∗
         WP (Loop : expr riscv_lang) @ E {{ Phi }}) -∗
     WP (Loop : expr riscv_lang) @ E {{ Phi }}.
   Proof.
@@ -5033,7 +5033,7 @@ Section WpCsrw2ProbeMc.
       (b1 : bool) (npc0 mst0 mstatus0 : mword 64)
       (mc : mword 32) (mcfg : mword 64)
       (pmpcfg0 : type_of_register pmpcfg_n) (pmar0 : list PMA_Region)
-      (mi0 : bool) (elp0 : mword 1) E (Phi : mval -> iProp Σ) :
+      (mi0 : bool) (elp0 : mword 1) E {dq : dfrac} (Phi : mval -> iProp Σ) :
     uint rs1 <> 0 ->
     m !! gpr_of_Z (uint rs1) = Some vrs1 ->
     eq_vec (_get_Misa_S misa0) ('b"1") = true ->
@@ -5066,7 +5066,7 @@ Section WpCsrw2ProbeMc.
     (R_bitvector_64 mideleg) ↦ᵣ mdv0 -∗ (R_bitvector_64 mstatus) ↦ᵣ mstatus0 -∗
     elp ↦ᵣ elp0 -∗ mcountinhibit ↦ᵣ mc -∗ minstretcfg ↦ᵣ mcfg -∗
     pmpcfg_n ↦ᵣ pmpcfg0 -∗ pma_regions ↦ᵣ pmar0 -∗ htif_tohost_base ↦ᵣ None -∗
-    ([∗ list] j ∈ seq 0 4, (pa_add (fetch_pa pc) j) ↦ₘ nth_byte w j) -∗
+    ([∗ list] j ∈ seq 0 4, (pa_add (fetch_pa pc) j) ↦ₘ{dq} nth_byte w j) -∗
     ▷ ( PC ↦ᵣ add_vec_int pc 4 -∗ gpr_file m -∗
         mcounteren ↦ᵣ legalize_mcounteren mcounteren0 vrs1 -∗ misa ↦ᵣ misa0 -∗
         nextPC ↦ᵣ add_vec_int pc 4 -∗ (R_bool minstret_increment) ↦ᵣ b1 -∗
@@ -5075,7 +5075,7 @@ Section WpCsrw2ProbeMc.
         (R_bitvector_64 mideleg) ↦ᵣ mdv0 -∗ (R_bitvector_64 mstatus) ↦ᵣ mstatus0 -∗
         elp ↦ᵣ elp0 -∗ mcountinhibit ↦ᵣ mc -∗ minstretcfg ↦ᵣ mcfg -∗
         pmpcfg_n ↦ᵣ pmpcfg0 -∗ pma_regions ↦ᵣ pmar0 -∗ htif_tohost_base ↦ᵣ None -∗
-        ([∗ list] j ∈ seq 0 4, (pa_add (fetch_pa pc) j) ↦ₘ nth_byte w j) -∗
+        ([∗ list] j ∈ seq 0 4, (pa_add (fetch_pa pc) j) ↦ₘ{dq} nth_byte w j) -∗
         WP (Loop : expr riscv_lang) @ E {{ Phi }}) -∗
     WP (Loop : expr riscv_lang) @ E {{ Phi }}.
   Proof.
