iris/WpGprLoad.v
@@ -245,7 +245,7 @@ Section WpLoadGpr.
       (mc : mword 32) (mcfg : mword 64)
       (mseccfg0 : mword 64) (pmpcfg0 : type_of_register pmpcfg_n)
       (pmar0 : list PMA_Region) (mi0a : bool) (elp0a : mword 1)
-      E (Φ : mval -> iProp Σ) :
+      E {dq : dfrac} (Φ : mval -> iProp Σ) :
     let offset := sign_extend' 64 imm_l in
     let ea := add_vec vrs1 offset in
     let a8 := zero_extend' 64 (subrange_vec_dec ea (xlen - 0 - 1) 0) in
@@ -279,7 +279,7 @@ Section WpLoadGpr.
     elp ↦ᵣ elp0a -∗ mseccfg ↦ᵣ mseccfg0 -∗ pmpcfg_n ↦ᵣ pmpcfg0 -∗ pma_regions ↦ᵣ pmar0 -∗
     mcountinhibit ↦ᵣ mc -∗ minstretcfg ↦ᵣ mcfg -∗ htif_tohost_base ↦ᵣ None -∗
     ([∗ list] j ∈ seq 0 8, (pa_add pa j) ↦ₘ nth_byte v j) -∗
-    ([∗ list] j ∈ seq 0 4, (pa_add (fetch_pa pc) j) ↦ₘ nth_byte w_l j) -∗
+    ([∗ list] j ∈ seq 0 4, (pa_add (fetch_pa pc) j) ↦ₘ{dq} nth_byte w_l j) -∗
     ▷ ( PC ↦ᵣ add_vec_int pc 4 -∗
         gpr_file (<[gpr_of_Z (uint rd) := regval_into_reg (extend_value false data2)]> m) -∗
         misa ↦ᵣ misa0 -∗
@@ -290,7 +290,7 @@ Section WpLoadGpr.
         elp ↦ᵣ elp0a -∗ mseccfg ↦ᵣ mseccfg0 -∗ pmpcfg_n ↦ᵣ pmpcfg0 -∗ pma_regions ↦ᵣ pmar0 -∗
         mcountinhibit ↦ᵣ mc -∗ minstretcfg ↦ᵣ mcfg -∗ htif_tohost_base ↦ᵣ None -∗
         ([∗ list] j ∈ seq 0 8, (pa_add pa j) ↦ₘ nth_byte v j) -∗
-        ([∗ list] j ∈ seq 0 4, (pa_add (fetch_pa pc) j) ↦ₘ nth_byte w_l j) -∗
+        ([∗ list] j ∈ seq 0 4, (pa_add (fetch_pa pc) j) ↦ₘ{dq} nth_byte w_l j) -∗
         WP (Loop : expr riscv_lang) @ E {{ Φ }}) -∗
     WP (Loop : expr riscv_lang) @ E {{ Φ }}.
   Proof.
