iris/WpGprLogic.v
@@ -203,7 +203,7 @@ Section WpOrGpr.
       (b1 : bool) (npc0 mst0 mstatus0 : mword 64)
       (mc : mword 32) (mcfg : mword 64)
       (pmpcfg0 : type_of_register pmpcfg_n) (pmar0 : list PMA_Region)
-      (mi0 : bool) (elp0 : mword 1) E (Phi : mval -> iProp Σ) :
+      (mi0 : bool) (elp0 : mword 1) E {dq : dfrac} (Phi : mval -> iProp Σ) :
     uint rs1 <> 0 -> uint rs2 <> 0 -> uint rd <> 0 ->
     m !! gpr_of_Z (uint rs1) = Some va ->
     m !! gpr_of_Z (uint rs2) = Some vb ->
@@ -228,7 +228,7 @@ Section WpOrGpr.
     (R_bitvector_64 mideleg) ↦ᵣ mdv0 -∗ (R_bitvector_64 mstatus) ↦ᵣ mstatus0 -∗
     elp ↦ᵣ elp0 -∗ mcountinhibit ↦ᵣ mc -∗ minstretcfg ↦ᵣ mcfg -∗
     pmpcfg_n ↦ᵣ pmpcfg0 -∗ pma_regions ↦ᵣ pmar0 -∗ htif_tohost_base ↦ᵣ None -∗
-    ([∗ list] j ∈ seq 0 4, (pa_add (fetch_pa pc) j) ↦ₘ nth_byte w j) -∗
+    ([∗ list] j ∈ seq 0 4, (pa_add (fetch_pa pc) j) ↦ₘ{dq} nth_byte w j) -∗
     ▷ ( PC ↦ᵣ add_vec_int pc 4 -∗
         gpr_file (<[gpr_of_Z (uint rd) := regval_into_reg (or_vec va vb)]> m) -∗
         misa ↦ᵣ misa0 -∗
@@ -238,7 +238,7 @@ Section WpOrGpr.
         (R_bitvector_64 mideleg) ↦ᵣ mdv0 -∗ (R_bitvector_64 mstatus) ↦ᵣ mstatus0 -∗
         elp ↦ᵣ elp0 -∗ mcountinhibit ↦ᵣ mc -∗ minstretcfg ↦ᵣ mcfg -∗
         pmpcfg_n ↦ᵣ pmpcfg0 -∗ pma_regions ↦ᵣ pmar0 -∗ htif_tohost_base ↦ᵣ None -∗
-        ([∗ list] j ∈ seq 0 4, (pa_add (fetch_pa pc) j) ↦ₘ nth_byte w j) -∗
+        ([∗ list] j ∈ seq 0 4, (pa_add (fetch_pa pc) j) ↦ₘ{dq} nth_byte w j) -∗
         WP (Loop : expr riscv_lang) @ E {{ Phi }}) -∗
     WP (Loop : expr riscv_lang) @ E {{ Phi }}.
   Proof.
@@ -478,7 +478,7 @@ Section WpAndGpr.
       (b1 : bool) (npc0 mst0 mstatus0 : mword 64)
       (mc : mword 32) (mcfg : mword 64)
       (pmpcfg0 : type_of_register pmpcfg_n) (pmar0 : list PMA_Region)
-      (mi0 : bool) (elp0 : mword 1) E (Phi : mval -> iProp Σ) :
+      (mi0 : bool) (elp0 : mword 1) E {dq : dfrac} (Phi : mval -> iProp Σ) :
     uint rs1 <> 0 -> uint rs2 <> 0 -> uint rd <> 0 ->
     m !! gpr_of_Z (uint rs1) = Some va ->
     m !! gpr_of_Z (uint rs2) = Some vb ->
@@ -503,7 +503,7 @@ Section WpAndGpr.
     (R_bitvector_64 mideleg) ↦ᵣ mdv0 -∗ (R_bitvector_64 mstatus) ↦ᵣ mstatus0 -∗
     elp ↦ᵣ elp0 -∗ mcountinhibit ↦ᵣ mc -∗ minstretcfg ↦ᵣ mcfg -∗
     pmpcfg_n ↦ᵣ pmpcfg0 -∗ pma_regions ↦ᵣ pmar0 -∗ htif_tohost_base ↦ᵣ None -∗
-    ([∗ list] j ∈ seq 0 4, (pa_add (fetch_pa pc) j) ↦ₘ nth_byte w j) -∗
+    ([∗ list] j ∈ seq 0 4, (pa_add (fetch_pa pc) j) ↦ₘ{dq} nth_byte w j) -∗
     ▷ ( PC ↦ᵣ add_vec_int pc 4 -∗
         gpr_file (<[gpr_of_Z (uint rd) := regval_into_reg (and_vec va vb)]> m) -∗
         misa ↦ᵣ misa0 -∗
@@ -513,7 +513,7 @@ Section WpAndGpr.
         (R_bitvector_64 mideleg) ↦ᵣ mdv0 -∗ (R_bitvector_64 mstatus) ↦ᵣ mstatus0 -∗
         elp ↦ᵣ elp0 -∗ mcountinhibit ↦ᵣ mc -∗ minstretcfg ↦ᵣ mcfg -∗
         pmpcfg_n ↦ᵣ pmpcfg0 -∗ pma_regions ↦ᵣ pmar0 -∗ htif_tohost_base ↦ᵣ None -∗
-        ([∗ list] j ∈ seq 0 4, (pa_add (fetch_pa pc) j) ↦ₘ nth_byte w j) -∗
+        ([∗ list] j ∈ seq 0 4, (pa_add (fetch_pa pc) j) ↦ₘ{dq} nth_byte w j) -∗
         WP (Loop : expr riscv_lang) @ E {{ Phi }}) -∗
     WP (Loop : expr riscv_lang) @ E {{ Phi }}.
   Proof.
@@ -755,7 +755,7 @@ Section WpOriGpr.
       (b1 : bool) (npc0 mst0 mstatus0 : mword 64)
       (mc : mword 32) (mcfg : mword 64)
       (pmpcfg0 : type_of_register pmpcfg_n) (pmar0 : list PMA_Region)
-      (mi0 : bool) (elp0 : mword 1) E (Phi : mval -> iProp Σ) :
+      (mi0 : bool) (elp0 : mword 1) E {dq : dfrac} (Phi : mval -> iProp Σ) :
     uint rs1 <> 0 -> uint rd <> 0 ->
     m !! gpr_of_Z (uint rs1) = Some va ->
     m !! gpr_of_Z (uint rd) = Some vd ->
@@ -779,7 +779,7 @@ Section WpOriGpr.
     (R_bitvector_64 mideleg) ↦ᵣ mdv0 -∗ (R_bitvector_64 mstatus) ↦ᵣ mstatus0 -∗
     elp ↦ᵣ elp0 -∗ mcountinhibit ↦ᵣ mc -∗ minstretcfg ↦ᵣ mcfg -∗
     pmpcfg_n ↦ᵣ pmpcfg0 -∗ pma_regions ↦ᵣ pmar0 -∗ htif_tohost_base ↦ᵣ None -∗
-    ([∗ list] j ∈ seq 0 4, (pa_add (fetch_pa pc) j) ↦ₘ nth_byte w j) -∗
+    ([∗ list] j ∈ seq 0 4, (pa_add (fetch_pa pc) j) ↦ₘ{dq} nth_byte w j) -∗
     ▷ ( PC ↦ᵣ add_vec_int pc 4 -∗
         gpr_file (<[gpr_of_Z (uint rd) := regval_into_reg (or_vec va (sign_extend' 64 imm))]> m) -∗
         misa ↦ᵣ misa0 -∗
@@ -789,7 +789,7 @@ Section WpOriGpr.
         (R_bitvector_64 mideleg) ↦ᵣ mdv0 -∗ (R_bitvector_64 mstatus) ↦ᵣ mstatus0 -∗
         elp ↦ᵣ elp0 -∗ mcountinhibit ↦ᵣ mc -∗ minstretcfg ↦ᵣ mcfg -∗
         pmpcfg_n ↦ᵣ pmpcfg0 -∗ pma_regions ↦ᵣ pmar0 -∗ htif_tohost_base ↦ᵣ None -∗
-        ([∗ list] j ∈ seq 0 4, (pa_add (fetch_pa pc) j) ↦ₘ nth_byte w j) -∗
+        ([∗ list] j ∈ seq 0 4, (pa_add (fetch_pa pc) j) ↦ₘ{dq} nth_byte w j) -∗
         WP (Loop : expr riscv_lang) @ E {{ Phi }}) -∗
     WP (Loop : expr riscv_lang) @ E {{ Phi }}.
   Proof.
